coq/exec/Nop.v
@@ -1,0 +1,128 @@
+Require Import syntax.
+Require Import alist.
+Require Import FMapWeakList.
+
+Require Import Coqlib.
+Require Import infrastructure.
+Require Import Metatheory.
+Import LLVMsyntax.
+Import LLVMinfra.
+
+Require Import sflib.
+
+Require Import TODO.
+
+Set Implicit Arguments.
+
+(* Get next nop id. Each id should be unique in Function. *)
+(* Should manually be extracted to proper Ocaml code. *)
+Parameter next_nop_id: blocks -> id.
+
+(* Search through blocks with target label, and insert nop. *)
+(* Logic adding nop is commented below. *)
+(* If there is multiple blocks with target label, it only inserts in FIRST block. *)
+Definition insert_nop (target:id) (bs:blocks): blocks :=
+  map
+    (fun stmts =>
+       let '(stmts_intro phinodes cmds terminator) := stmts in
+
+       (* after a phinode *)
+       let phinodes_valid :=
+           List.existsb
+             (fun phinode => if eq_atom_dec (getPhiNodeID phinode) target then true else false)
+             phinodes
+       in
+       let cmds :=
+           if phinodes_valid
+           then insert_at 0 (insn_nop (next_nop_id bs)) cmds
+           else cmds
+       in
+
+       (* after a command *)
+       let cmds_idx :=
+           find_index
+             cmds
+             (fun c => if eq_atom_dec (getCmdLoc c) target then true else false)
+       in
+       let cmds :=
+           match cmds_idx with
+           | None => cmds
+           | Some idx => insert_at (idx + 1) (insn_nop (next_nop_id bs)) cmds
+           end
+       in
+
+       stmts_intro phinodes cmds terminator)
+    bs.
+
+(* Insert multiple nops in blocks. *)
+Definition insert_nops (targets:list id) (bs:blocks): blocks :=
+  List.fold_left (flip insert_nop) targets bs.
+
+(* TODO: how about defining with filters? *)
+Inductive nop_cmds: forall (cmds_src cmds_tgt:cmds), Prop :=
+| nop_cmds_nil:
+    nop_cmds nil nil
+| nop_cmds_cons
+    c cmds_src cmds_tgt
+    (NOP: nop_cmds cmds_src cmds_tgt):
+    nop_cmds (c::cmds_src) (c::cmds_tgt)
+| nop_cmds_src
+    id cmds_src cmds_tgt
+    (NOP: nop_cmds cmds_src cmds_tgt):
+    nop_cmds ((insn_nop id)::cmds_src) cmds_tgt
+| nop_cmds_tgt
+    id cmds_src cmds_tgt
+    (NOP: nop_cmds cmds_src cmds_tgt):
+    nop_cmds cmds_src ((insn_nop id)::cmds_tgt)
+.
+
+Definition nop_blocks (blocks_src blocks_tgt:blocks): Prop :=
+  forall bid,
+    lift2_option
+      (fun stmts_src stmts_tgt =>
+         let '(stmts_intro phinodes_src cmds_src terminator_src) := stmts_src in
+         let '(stmts_intro phinodes_tgt cmds_tgt terminator_tgt) := stmts_tgt in
+         phinodes_src = phinodes_tgt /\
+         nop_cmds cmds_src cmds_tgt /\
+         terminator_src = terminator_tgt)
+    (lookupAL _ blocks_src bid)
+    (lookupAL _ blocks_tgt bid).
+
+Lemma lookupAL_mapAL A B i (f:A -> B) l:
+  lookupAL _ (map f l) i = option_map f (lookupAL _ l i).
+Proof.
+Admitted.
+
+Lemma insert_nop_spec1 id bs:
+  nop_blocks bs (insert_nop id bs).
+Proof.
+  ii. unfold insert_nop. rewrite lookupAL_mapAL.
+  destruct (lookupAL _ bs bid); simpl in *; auto.
+  destruct s; splits; auto.
+  repeat
+    match goal with
+    | [|- context[match ?c with | Some _ => _ | None => _ end]] => destruct c
+    | [|- context[if ?c then _ else _]] => destruct c
+    end.
+  - admit.
+  - admit.
+  - admit.
+  - admit.
+Admitted.
+
+Lemma insert_nop_spec2 id bs:
+  nop_blocks (insert_nop id bs) bs.
+Proof.
+  ii. unfold insert_nop. rewrite lookupAL_mapAL.
+  destruct (lookupAL _ bs bid); simpl in *; auto.
+  destruct s; splits; auto.
+  repeat
+    match goal with
+    | [|- context[match ?c with | Some _ => _ | None => _ end]] => destruct c
+    | [|- context[if ?c then _ else _]] => destruct c
+    end.
+  - admit.
+  - admit.
+  - admit.
+  - admit.
+Admitted.
